---
title: '2DGS梯度推导'
date: 2024-11-05
permalink: /posts/2024/11/2DGS梯度推导/
tags:
  - 2DGS
---

https://en.wikipedia.org/wiki/Matrix_calculus#Scalar-by-vector_identities

# Ray-splat points

$$
\mathbf{x}=(x z, y z, z, 1)^{\mathrm{T}}=\mathbf{W} P(u, v)=\mathbf{W H}(u, v, 1,1)^{\mathrm{T}}
$$

$$
\hat{\mathbf{x}}=(x, y, z)^{\mathrm{T}}=(\frac{1}{z}, \frac{1}{z}, 1)\mathbf{W} P(u, v)
$$

# Depth

## Mean depth

$$
D=\sum_i \omega_i z_i
$$

where 

$$
\omega_i=T_i \alpha_i \hat{\mathcal{G}}_i(\mathbf{u}(\mathbf{x}))
$$

 is the weight contribution of the 

$i$

-th Gaussian and 

$$
T_i=\prod_{j=1}^{i-1}\left(1-\alpha_j \hat{\mathcal{G}}_j(\mathbf{u}(\mathbf{x}))\right)
$$

 measures its visibility.

- Relative variables
  - $$
    z_i
    $$
  - $$
    \omega_i
    $$

### Calculate 
$$
z_i
$$


$$
\frac{\partial z_{\text {mean }}}{\partial z_i}=\omega_i
$$

$$
\frac{\partial L}{\partial z_i}=\frac{\partial L}{D}\frac{D}{\partial z_i}=\frac{\partial L}{D}\omega_i
$$

### Calculate 
$$
\omega_i
$$


$$
\frac{\partial z_{\text {mean }}}{\partial \omega_i}= z_i
$$

$$
\frac{\partial L}{\partial \omega_i}=\frac{\partial L}{D}\frac{D}{\partial \omega_i}=\frac{\partial L}{D}z_i
$$

### Calculate 
$$
\alpha_i
$$

$$
\frac{\partial T_i}{\partial \alpha_i} =  T_{i-1} \left(-\hat{\mathcal{G}}_{i-1}(\mathbf{u}(\mathbf{x}))\right)
$$


$$
\frac{\partial \omega_i}{\partial \alpha_i}= T_i \hat{\mathcal{G}}_i(\mathbf{u}(\mathbf{x})) +  \alpha_i \hat{\mathcal{G}}_i(\mathbf{u}(\mathbf{x})) \frac{\partial T_i}{\partial \alpha_i}\\
= T_i \hat{\mathcal{G}}_i(\mathbf{u}(\mathbf{x})) - \alpha_i T_{i-1} \hat{\mathcal{G}}_{i-1}(\mathbf{u}(\mathbf{x})) \hat{\mathcal{G}}_i(\mathbf{u}(\mathbf{x}))
$$

# Distortion loss

$$
\begin{aligned}
&\begin{aligned}
\mathcal{Dist} & =\sum_{i=0}^{N-1} \sum_{j=0}^{i-1} \omega_i \omega_j\left(m_i-m_j\right)^2 \\
& =\sum_{i=0}^{N-1} \omega_i\left(m_i^2 \sum_{j=0}^{i-1} \omega_j+\sum_{j=0}^{i-1} \omega_j m_j^2-2 m_i \sum_{j=0}^{i-1} \omega_j m_j\right) \\
& =\sum_{i=0}^{N-1} \omega_i\left(m_i^2 A_{i-1}+D_{i-1}^2-2 m_i D_{i-1}\right)
\end{aligned}\\
&\text { where } A_i=\sum_{j=0}^{i} \omega_j, D_i=\sum_{j=0}^{i} \omega_j m_j \text { and } D_i^2=\sum_{j=0}^{i} \omega_j m_j^2 \text {. }
\end{aligned}
$$

$$
A_i=\sum_{j=0}^{i} \omega_j =\sum_{j=0}^{i} \alpha_j \hat{\mathcal{G}}_j(\mathbf{u}(\mathbf{x})) T_j = 1.0 - T_i = 1.0 - \prod_{j=1}^{i}\left(1-\alpha_j \hat{\mathcal{G}}_j(\mathbf{u}(\mathbf{x}))\right)
$$

$$
\frac{\partial \mathcal{Dist}}{\partial m_i}=\omega_i * 2 * m_i * A_{i-1} - 2 D_{i-1} = 2 (\omega_i * m_i * A_{i-1} - D_{i-1})
$$

$$
\frac{\partial \mathcal{Dist}}{\partial \omega_i}=m_i^2 A_{i-1}+D_{i-1}^2-2 m_i D_{i-1}
$$

$$
\frac{\partial \mathcal{Dist}}{\partial \alpha_i}=\frac{\partial L}{\partial \omega_i} \frac{\partial \omega_i}{\partial \alpha_i}
$$